Nerodia.lean
@@ -4,6 +4,7 @@ Released under Apache 2.0 license as described in the file LICENSE.
 Authors: Mac Malone
 -/
 module
+public import Nerodia.Data
 public import Nerodia.Basic
 public import Nerodia.Compiler.ModuleConfig.Basic
 public meta import Nerodia.Compiler.ModuleConfig.Extension
