Nerodia/Data/Addr.lean
@@ -1,0 +1,85 @@
+/-
+Copyright (c) 2026 Lean FRO. All rights reserved.
+Released under Apache 2.0 license as described in the file LICENSE.
+Authors: Mac Malone
+-/
+module
+
+/-! # Pointer Addresses -/
+
+namespace Nerodia
+
+/-! ## Nullable Pointer Address -/
+
+/-- A pointer address. May be {lit}`NULL`. -/
+public structure NullableAddr where
+  private ofUSizeUnsafe ::
+    toUSize : USize
+    deriving DecidableEq
+
+namespace NullableAddr
+
+/-- The address of a null pointer (i.e., {lit}`NULL` in C). -/
+@[inline] public protected def null : NullableAddr :=
+  ⟨0⟩ -- `NULL = 0` on Lean-supported platforms
+
+public instance : Inhabited NullableAddr := ⟨NullableAddr.null⟩
+
+public abbrev IsNull (self : NullableAddr) : Prop :=
+  self = NullableAddr.null
+
+@[simp] public theorem isNull_null : IsNull NullableAddr.null := by rfl
+
+public abbrev toNat (self : NullableAddr) : Nat :=
+  self.toUSize.toNat
+
+end NullableAddr
+
+/-! ## Null -/
+
+/-- The type of the null pointer constant (i.e., {lit}`NULL` in C). -/
+-- `Null` is defined as a subtype of `NullableAddr` instead of a singleton
+-- inductive in order to retain a `USize` runtime representation, which is
+-- necessary for the function signature of `PyMethNoArgs`.
+public structure Null where
+  addr : NullableAddr
+  isNull_addr : addr.IsNull
+
+namespace Null
+
+public theorem addr_inj : addr a = addr b ↔ a = b := by
+  cases a; cases b; simp
+
+/-- The null pointer constant (i.e., {lit}`NULL` in C). -/
+@[inline] public def null : Null :=
+  ⟨NullableAddr.null, rfl⟩
+
+public instance : Inhabited Null := ⟨null⟩
+public instance : Coe Null NullableAddr := ⟨fun _ => NullableAddr.null⟩
+
+public instance : Subsingleton Null where
+  allEq a b := by simp [← addr_inj, a.isNull_addr, b.isNull_addr]
+
+end Null
+
+export Null (null)
+
+/-! ## Non-Null Pointer Address -/
+
+/-- A pointer address. -/
+public structure Addr extends NullableAddr where
+  ofNullableAddr ::
+    not_isNull : ¬ toNullableAddr.IsNull
+    deriving DecidableEq
+
+namespace Addr
+
+public instance : Nonempty Addr :=
+  ⟨⟨⟨1⟩, by simp [NullableAddr.null, ← USize.toNat_inj]⟩⟩
+
+public instance : Coe Addr NullableAddr := ⟨toNullableAddr⟩
+
+public theorem toNullableAddr_inj : toNullableAddr a = toNullableAddr b ↔ a = b := by
+  cases a; cases b; simp
+
+end Addr
