Nerodia/Data/CPtr.lean
@@ -1,0 +1,86 @@
+/-
+Copyright (c) 2026 Lean FRO. All rights reserved.
+Released under Apache 2.0 license as described in the file LICENSE.
+Authors: Mac Malone
+-/
+module
+public import Nerodia.Data.Addr
+
+/-! # Raw C Pointers -/
+
+namespace Nerodia
+
+/-! ## Nullable Pointers -/
+
+/--
+A raw C pointer. May be {lit}`NULL`.
+
+**Not memory safe.** The pointer's lifetime must be manually managed.
+It is not managed by Lean. Nerodia handles this within its API, and users are
+not expected to manage {name}`NullableCPtr` objects manually.
+-/
+public structure NullableCPtr (α : Type u) : Type where
+  private ofNullableAddrUnsafe ::
+    nullableAddr : NullableAddr
+    nonempty_of_not_isNull_nullableAddr (h : ¬ nullableAddr.IsNull) : Nonempty α
+    deriving DecidableEq
+
+namespace NullableCPtr
+
+@[inline] def ofAddrUnsafe [Nonempty α] (addr : Addr) : NullableCPtr α :=
+  ofNullableAddrUnsafe addr fun _ => inferInstance
+
+public theorem nullableAddr_inj : nullableAddr a = nullableAddr b ↔ a = b := by
+  cases a; cases b; simp
+
+@[inline] public protected def null : NullableCPtr α :=
+  ⟨null, by simp⟩
+
+public instance : Coe Null (NullableCPtr α) := ⟨fun _ => NullableCPtr.null⟩
+public instance : Inhabited (NullableCPtr α) := ⟨null⟩
+
+public abbrev IsNull (self : NullableCPtr α) : Prop :=
+  self.nullableAddr.IsNull
+
+@[simp, grind .] public theorem isNull_null : IsNull (α := α) null := by rfl
+
+public theorem nonempty_of_not_isNull
+  {p : NullableCPtr α} (h : ¬ IsNull p) : Nonempty α
+:= p.nonempty_of_not_isNull_nullableAddr <| by simpa [← nullableAddr_inj] using h
+
+end NullableCPtr
+
+/-! ## Non-Null Pointers -/
+
+/--
+A raw C pointer.
+
+**Not memory safe.** The pointer's lifetime must be manually managed.
+It is not managed by Lean. Nerodia handles this within its API, and users are
+not expected to manage {name}`CPtr` objects manually.
+-/
+public structure CPtr (α : Type u) extends NullableCPtr α where
+  ofNullableCPtr ::
+    not_isNull : ¬ toNullableCPtr.IsNull
+    deriving DecidableEq
+
+namespace CPtr
+
+public instance : Coe (CPtr α) (NullableCPtr α) := ⟨toNullableCPtr⟩
+
+public noncomputable def ofAddrNoncomputable [Nonempty α] (addr : Addr) : CPtr α :=
+  ofNullableCPtr (.ofAddrUnsafe addr) addr.not_isNull
+
+public instance [Nonempty α] : Nonempty (CPtr α) :=
+  ⟨ofAddrNoncomputable Classical.ofNonempty⟩
+
+@[inline] public def addr (self : CPtr α) : Addr :=
+  .ofNullableAddr self.nullableAddr self.not_isNull
+
+public theorem addr_inj : addr a = addr b ↔ a = b := by
+  cases a; cases b; simp [← NullableCPtr.nullableAddr_inj, addr]
+
+public theorem nonempty {self : CPtr α} : Nonempty α :=
+  self.toNullableCPtr.nonempty_of_not_isNull self.not_isNull
+
+end CPtr
